<?xml version="1.0"?>
<rdf:RDF xmlns="http://www.semanticweb.org/prosy/ontologies/2024/3/Airline_Reviews_Ontology#"
     xml:base="http://www.semanticweb.org/prosy/ontologies/2024/3/Airline_Reviews_Ontology"
     xmlns:owl="http://www.w3.org/2002/07/owl#"
     xmlns:rdf="http://www.w3.org/1999/02/22-rdf-syntax-ns#"
     xmlns:xml="http://www.w3.org/XML/1998/namespace"
     xmlns:xsd="http://www.w3.org/2001/XMLSchema#"
     xmlns:rdfs="http://www.w3.org/2000/01/rdf-schema#"
     xmlns:Airline_Reviews_Ontology="http://www.semanticweb.org/prosy/ontologies/2024/3/Airline_Reviews_Ontology#">
    <owl:Ontology rdf:about="http://www.semanticweb.org/prosy/ontologies/2024/3/Airline_Reviews_Ontology">
        <rdfs:comment>This ontology is designed to structure and relate information obtained from customer reviews of Qatar Airways and Ryanair airlines, facilitating the analysis and comparison of flight services through different parameters such as comfort, cabin service, and general customer satisfaction. customer.</rdfs:comment>
    </owl:Ontology>
    


    <!-- 
    ///////////////////////////////////////////////////////////////////////////////////////
    //
    // Annotation properties
    //
    ///////////////////////////////////////////////////////////////////////////////////////
     -->


    


    <!-- http://www.w3.org/2000/01/rdf-schema#sameAs -->


    <owl:AnnotationProperty rdf:about="http://www.w3.org/2000/01/rdf-schema#sameAs"/>
    


    <!-- 
    ///////////////////////////////////////////////////////////////////////////////////////
    //
    // Object Properties
    //
    ///////////////////////////////////////////////////////////////////////////////////////
     -->


    


    <!-- http://www.semanticweb.org/prosy/ontologies/2024/3/Airline_Reviews_Ontology#ObjectProperty -->


    <owl:ObjectProperty rdf:about="http://www.semanticweb.org/prosy/ontologies/2024/3/Airline_Reviews_Ontology#ObjectProperty">
        <rdfs:range rdf:resource="http://www.semanticweb.org/prosy/ontologies/2024/3/Airline_Reviews_Ontology#ServiceRatings"/>
        <rdfs:comment>Links a review to the services evaluated</rdfs:comment>
        <rdfs:label>objectProperty</rdfs:label>
    </owl:ObjectProperty>
    


    <!-- http://www.semanticweb.org/prosy/ontologies/2024/3/Airline_Reviews_Ontology#fliesFromTo -->


    <owl:ObjectProperty rdf:about="http://www.semanticweb.org/prosy/ontologies/2024/3/Airline_Reviews_Ontology#fliesFromTo">
        <rdfs:range rdf:resource="http://www.semanticweb.org/prosy/ontologies/2024/3/Airline_Reviews_Ontology#FlightDetails"/>
        <rdfs:comment>Connects a flight review with its departure and destination airports</rdfs:comment>
        <rdfs:label>filesFromTo</rdfs:label>
    </owl:ObjectProperty>
    


    <!-- http://www.semanticweb.org/prosy/ontologies/2024/3/Airline_Reviews_Ontology#hasAuthor -->


    <owl:ObjectProperty rdf:about="http://www.semanticweb.org/prosy/ontologies/2024/3/Airline_Reviews_Ontology#hasAuthor">
        <rdfs:domain rdf:resource="http://www.semanticweb.org/prosy/ontologies/2024/3/Airline_Reviews_Ontology#Identifier"/>
        <rdfs:range rdf:resource="http://www.semanticweb.org/prosy/ontologies/2024/3/Airline_Reviews_Ontology#Author"/>
        <rdfs:comment>Connects a flight review with its departure and destination airports</rdfs:comment>
        <rdfs:label>hasAuthor</rdfs:label>
    </owl:ObjectProperty>
    


    <!-- http://www.semanticweb.org/prosy/ontologies/2024/3/Airline_Reviews_Ontology#hasFlightDetails -->


    <owl:ObjectProperty rdf:about="http://www.semanticweb.org/prosy/ontologies/2024/3/Airline_Reviews_Ontology#hasFlightDetails">
        <rdf:type rdf:resource="http://www.w3.org/2002/07/owl#TransitiveProperty"/>
        <rdfs:domain rdf:resource="http://www.semanticweb.org/prosy/ontologies/2024/3/Airline_Reviews_Ontology#Author"/>
        <rdfs:range rdf:resource="http://www.semanticweb.org/prosy/ontologies/2024/3/Airline_Reviews_Ontology#FlightDetails"/>
        <rdfs:comment>Associates a review with specific flight details</rdfs:comment>
        <rdfs:label>hasFlightDetails</rdfs:label>
    </owl:ObjectProperty>
    


    <!-- http://www.semanticweb.org/prosy/ontologies/2024/3/Airline_Reviews_Ontology#hasRating -->


    <owl:ObjectProperty rdf:about="http://www.semanticweb.org/prosy/ontologies/2024/3/Airline_Reviews_Ontology#hasRating">
        <rdfs:domain rdf:resource="http://www.semanticweb.org/prosy/ontologies/2024/3/Airline_Reviews_Ontology#Identifier"/>
        <rdfs:range rdf:resource="http://www.semanticweb.org/prosy/ontologies/2024/3/Airline_Reviews_Ontology#Ratings"/>
        <rdfs:comment>Connects a review to the ratings it includes</rdfs:comment>
        <rdfs:label>hasRating</rdfs:label>
    </owl:ObjectProperty>
    


    <!-- http://www.semanticweb.org/prosy/ontologies/2024/3/Airline_Reviews_Ontology#hasRecommendation -->


    <owl:ObjectProperty rdf:about="http://www.semanticweb.org/prosy/ontologies/2024/3/Airline_Reviews_Ontology#hasRecommendation">
        <rdfs:range rdf:resource="http://www.semanticweb.org/prosy/ontologies/2024/3/Airline_Reviews_Ontology#Recommendation"/>
        <rdfs:comment>Relates a review to its recommendation status</rdfs:comment>
        <rdfs:label>hasRecommendation</rdfs:label>
    </owl:ObjectProperty>
    


    <!-- http://www.semanticweb.org/prosy/ontologies/2024/3/Airline_Reviews_Ontology#hasSeat -->


    <owl:ObjectProperty rdf:about="http://www.semanticweb.org/prosy/ontologies/2024/3/Airline_Reviews_Ontology#hasSeat">
        <rdfs:domain rdf:resource="http://www.semanticweb.org/prosy/ontologies/2024/3/Airline_Reviews_Ontology#AircraftDetails"/>
        <rdfs:range rdf:resource="http://www.semanticweb.org/prosy/ontologies/2024/3/Airline_Reviews_Ontology#SeatDetails"/>
        <rdfs:comment>Connects a review to the type of seat described in the review</rdfs:comment>
        <rdfs:label>hasSeat</rdfs:label>
    </owl:ObjectProperty>
    


    <!-- http://www.semanticweb.org/prosy/ontologies/2024/3/Airline_Reviews_Ontology#offersAmenities -->


    <owl:ObjectProperty rdf:about="http://www.semanticweb.org/prosy/ontologies/2024/3/Airline_Reviews_Ontology#offersAmenities">
        <rdfs:range rdf:resource="http://www.semanticweb.org/prosy/ontologies/2024/3/Airline_Reviews_Ontology#Amenities"/>
        <rdfs:comment>Associates a review with the amenities discussed within it</rdfs:comment>
        <rdfs:label>offersAmenities</rdfs:label>
    </owl:ObjectProperty>
    


    <!-- http://www.semanticweb.org/prosy/ontologies/2024/3/Airline_Reviews_Ontology#operatedBy -->


    <owl:ObjectProperty rdf:about="http://www.semanticweb.org/prosy/ontologies/2024/3/Airline_Reviews_Ontology#operatedBy">
        <rdf:type rdf:resource="http://www.w3.org/2002/07/owl#TransitiveProperty"/>
        <rdfs:domain rdf:resource="http://www.semanticweb.org/prosy/ontologies/2024/3/Airline_Reviews_Ontology#AircraftDetails"/>
        <rdfs:range rdf:resource="http://www.semanticweb.org/prosy/ontologies/2024/3/Airline_Reviews_Ontology#FlightDetails"/>
        <rdfs:comment>operate flying</rdfs:comment>
        <rdfs:label>operate by</rdfs:label>
    </owl:ObjectProperty>
    


    <!-- http://www.semanticweb.org/prosy/ontologies/2024/3/Airline_Reviews_Ontology#usesAircraft -->


    <owl:ObjectProperty rdf:about="http://www.semanticweb.org/prosy/ontologies/2024/3/Airline_Reviews_Ontology#usesAircraft">
        <rdfs:domain rdf:resource="http://www.semanticweb.org/prosy/ontologies/2024/3/Airline_Reviews_Ontology#Identifier"/>
        <rdfs:range rdf:resource="http://www.semanticweb.org/prosy/ontologies/2024/3/Airline_Reviews_Ontology#AircraftDetails"/>
        <rdfs:comment>Associates a review with the aircraft used for the flight</rdfs:comment>
        <rdfs:label>usesAircraft</rdfs:label>
    </owl:ObjectProperty>
    


    <!-- 
    ///////////////////////////////////////////////////////////////////////////////////////
    //
    // Data properties
    //
    ///////////////////////////////////////////////////////////////////////////////////////
     -->


    


    <!-- http://www.semanticweb.org/prosy/ontologies/2024/3/Airline_Reviews_Ontology#authorName -->


    <owl:DatatypeProperty rdf:about="http://www.semanticweb.org/prosy/ontologies/2024/3/Airline_Reviews_Ontology#authorName">
        <rdfs:subPropertyOf rdf:resource="http://www.semanticweb.org/prosy/ontologies/2024/3/Airline_Reviews_Ontology#idNumber"/>
        <rdfs:domain rdf:resource="http://www.semanticweb.org/prosy/ontologies/2024/3/Airline_Reviews_Ontology#Author"/>
        <rdfs:range rdf:resource="http://www.w3.org/2001/XMLSchema#string"/>
        <rdfs:comment>The name of the author of the review</rdfs:comment>
        <rdfs:label>authorName</rdfs:label>
    </owl:DatatypeProperty>
    


    <!-- http://www.semanticweb.org/prosy/ontologies/2024/3/Airline_Reviews_Ontology#comfortRating -->


    <owl:DatatypeProperty rdf:about="http://www.semanticweb.org/prosy/ontologies/2024/3/Airline_Reviews_Ontology#comfortRating">
        <rdfs:domain rdf:resource="http://www.semanticweb.org/prosy/ontologies/2024/3/Airline_Reviews_Ontology#SeatDetails"/>
        <rdfs:range rdf:resource="http://www.w3.org/2001/XMLSchema#integer"/>
        <rdfs:comment>The rating for seat comfort provided in the review</rdfs:comment>
        <rdfs:label>comfortRating</rdfs:label>
    </owl:DatatypeProperty>
    


    <!-- http://www.semanticweb.org/prosy/ontologies/2024/3/Airline_Reviews_Ontology#flightDate -->


    <owl:DatatypeProperty rdf:about="http://www.semanticweb.org/prosy/ontologies/2024/3/Airline_Reviews_Ontology#flightDate">
        <rdf:type rdf:resource="http://www.w3.org/2002/07/owl#FunctionalProperty"/>
        <rdfs:domain rdf:resource="http://www.semanticweb.org/prosy/ontologies/2024/3/Airline_Reviews_Ontology#FlightTimeliness"/>
        <rdfs:range rdf:resource="http://www.w3.org/2001/XMLSchema#dateTime"/>
        <rdfs:comment>The date of the flight being reviewed</rdfs:comment>
        <rdfs:label>flightDate</rdfs:label>
    </owl:DatatypeProperty>
    


    <!-- http://www.semanticweb.org/prosy/ontologies/2024/3/Airline_Reviews_Ontology#hasCabinStaffServiceRating -->


    <owl:DatatypeProperty rdf:about="http://www.semanticweb.org/prosy/ontologies/2024/3/Airline_Reviews_Ontology#hasCabinStaffServiceRating">
        <rdfs:domain rdf:resource="http://www.semanticweb.org/prosy/ontologies/2024/3/Airline_Reviews_Ontology#Identifier"/>
        <rdfs:range rdf:resource="http://www.w3.org/2001/XMLSchema#decimal"/>
        <rdfs:comment>ha scabin staf f service rating</rdfs:comment>
        <rdfs:label>hasCabinStaffServiceRating</rdfs:label>
    </owl:DatatypeProperty>
    


    <!-- http://www.semanticweb.org/prosy/ontologies/2024/3/Airline_Reviews_Ontology#hasRecommendationStatus -->


    <owl:DatatypeProperty rdf:about="http://www.semanticweb.org/prosy/ontologies/2024/3/Airline_Reviews_Ontology#hasRecommendationStatus">
        <rdfs:comment>recommendation status data</rdfs:comment>
        <rdfs:label>hasRecommendationStatus</rdfs:label>
    </owl:DatatypeProperty>
    


    <!-- http://www.semanticweb.org/prosy/ontologies/2024/3/Airline_Reviews_Ontology#idNumber -->


    <owl:DatatypeProperty rdf:about="http://www.semanticweb.org/prosy/ontologies/2024/3/Airline_Reviews_Ontology#idNumber">
        <rdf:type rdf:resource="http://www.w3.org/2002/07/owl#FunctionalProperty"/>
        <rdfs:domain rdf:resource="http://www.semanticweb.org/prosy/ontologies/2024/3/Airline_Reviews_Ontology#Identifier"/>
        <rdfs:range rdf:resource="http://www.w3.org/2001/XMLSchema#string"/>
        <rdfs:comment>he number when the id was published</rdfs:comment>
        <rdfs:label>idNumber</rdfs:label>
    </owl:DatatypeProperty>
    


    <!-- http://www.semanticweb.org/prosy/ontologies/2024/3/Airline_Reviews_Ontology#overallRating -->


    <owl:DatatypeProperty rdf:about="http://www.semanticweb.org/prosy/ontologies/2024/3/Airline_Reviews_Ontology#overallRating">
        <rdfs:domain rdf:resource="http://www.semanticweb.org/prosy/ontologies/2024/3/Airline_Reviews_Ontology#Identifier"/>
        <rdfs:range rdf:resource="http://www.w3.org/2001/XMLSchema#decimal"/>
        <rdfs:comment>The overall rating given in the review</rdfs:comment>
        <rdfs:label>overallRating</rdfs:label>
    </owl:DatatypeProperty>
    


    <!-- http://www.semanticweb.org/prosy/ontologies/2024/3/Airline_Reviews_Ontology#recommendationStatus -->


    <owl:DatatypeProperty rdf:about="http://www.semanticweb.org/prosy/ontologies/2024/3/Airline_Reviews_Ontology#recommendationStatus">
        <rdfs:domain rdf:resource="http://www.semanticweb.org/prosy/ontologies/2024/3/Airline_Reviews_Ontology#Identifier"/>
        <rdfs:range rdf:resource="http://www.w3.org/2001/XMLSchema#boolean"/>
        <rdfs:comment>Indicates whether the review recommends the airline service</rdfs:comment>
        <rdfs:label>recommendationStatus</rdfs:label>
    </owl:DatatypeProperty>
    


    <!-- http://www.semanticweb.org/prosy/ontologies/2024/3/Airline_Reviews_Ontology#reviewDate -->


    <owl:DatatypeProperty rdf:about="http://www.semanticweb.org/prosy/ontologies/2024/3/Airline_Reviews_Ontology#reviewDate">
        <rdf:type rdf:resource="http://www.w3.org/2002/07/owl#FunctionalProperty"/>
        <rdfs:domain rdf:resource="http://www.semanticweb.org/prosy/ontologies/2024/3/Airline_Reviews_Ontology#Identifier"/>
        <rdfs:range rdf:resource="http://www.w3.org/2001/XMLSchema#dateTime"/>
        <rdfs:comment>he date when the id was published</rdfs:comment>
        <rdfs:label>idDate</rdfs:label>
    </owl:DatatypeProperty>
    


    <!-- 
    ///////////////////////////////////////////////////////////////////////////////////////
    //
    // Classes
    //
    ///////////////////////////////////////////////////////////////////////////////////////
     -->


    


    <!-- http://www.semanticweb.org/prosy/ontologies/2024/3/Airline_Reviews_Ontology#AircraftDetails -->


    <owl:Class rdf:about="http://www.semanticweb.org/prosy/ontologies/2024/3/Airline_Reviews_Ontology#AircraftDetails">
        <rdfs:comment>Details about the aircraft used for the flight, such as the type and model</rdfs:comment>
        <rdfs:label>Aircraft Details</rdfs:label>
    </owl:Class>
    


    <!-- http://www.semanticweb.org/prosy/ontologies/2024/3/Airline_Reviews_Ontology#AircraftType -->


    <owl:Class rdf:about="http://www.semanticweb.org/prosy/ontologies/2024/3/Airline_Reviews_Ontology#AircraftType">
        <rdfs:subClassOf rdf:resource="http://www.semanticweb.org/prosy/ontologies/2024/3/Airline_Reviews_Ontology#AircraftDetails"/>
        <rdfs:comment>The type of aircraft used, such as Boeing 787 or Airbus A320</rdfs:comment>
        <rdfs:label>Aircraft Type</rdfs:label>
    </owl:Class>
    


    <!-- http://www.semanticweb.org/prosy/ontologies/2024/3/Airline_Reviews_Ontology#Amenities -->


    <owl:Class rdf:about="http://www.semanticweb.org/prosy/ontologies/2024/3/Airline_Reviews_Ontology#Amenities">
        <rdfs:comment>Additional comfort and convenience features offered to passengers during the flight</rdfs:comment>
        <rdfs:label>Amenities</rdfs:label>
    </owl:Class>
    


    <!-- http://www.semanticweb.org/prosy/ontologies/2024/3/Airline_Reviews_Ontology#AmenityAvailability -->


    <owl:Class rdf:about="http://www.semanticweb.org/prosy/ontologies/2024/3/Airline_Reviews_Ontology#AmenityAvailability">
        <rdfs:subClassOf rdf:resource="http://www.semanticweb.org/prosy/ontologies/2024/3/Airline_Reviews_Ontology#Amenities"/>
        <rdfs:comment>Specifies whether specific amenities are available on the flight, such as extra legroom or in-flight meals</rdfs:comment>
        <rdfs:label>Amenity Availability</rdfs:label>
    </owl:Class>
    


    <!-- http://www.semanticweb.org/prosy/ontologies/2024/3/Airline_Reviews_Ontology#Author -->


    <owl:Class rdf:about="http://www.semanticweb.org/prosy/ontologies/2024/3/Airline_Reviews_Ontology#Author">
        <rdfs:comment>The person who wrote the review. Includes name and country</rdfs:comment>
        <rdfs:label>Author</rdfs:label>
    </owl:Class>
    


    <!-- http://www.semanticweb.org/prosy/ontologies/2024/3/Airline_Reviews_Ontology#AuthorCountry -->


    <owl:Class rdf:about="http://www.semanticweb.org/prosy/ontologies/2024/3/Airline_Reviews_Ontology#AuthorCountry">
        <rdfs:subClassOf rdf:resource="http://www.semanticweb.org/prosy/ontologies/2024/3/Airline_Reviews_Ontology#Author"/>
        <owl:disjointWith rdf:resource="http://www.semanticweb.org/prosy/ontologies/2024/3/Airline_Reviews_Ontology#AuthorName"/>
        <rdfs:comment>he country where the author resides or from which they wrote the review</rdfs:comment>
        <rdfs:label>Author Country</rdfs:label>
    </owl:Class>
    


    <!-- http://www.semanticweb.org/prosy/ontologies/2024/3/Airline_Reviews_Ontology#AuthorName -->


    <owl:Class rdf:about="http://www.semanticweb.org/prosy/ontologies/2024/3/Airline_Reviews_Ontology#AuthorName">
        <rdfs:subClassOf rdf:resource="http://www.semanticweb.org/prosy/ontologies/2024/3/Airline_Reviews_Ontology#Author"/>
        <rdfs:comment>The name of the author of the review</rdfs:comment>
        <rdfs:label>Author Name</rdfs:label>
    </owl:Class>
    


    <!-- http://www.semanticweb.org/prosy/ontologies/2024/3/Airline_Reviews_Ontology#BaggageHandling -->


    <owl:Class rdf:about="http://www.semanticweb.org/prosy/ontologies/2024/3/Airline_Reviews_Ontology#BaggageHandling">
        <rdfs:comment>The process and efficiency of how an airline handles passenger luggage, from check-in to collection at the destination</rdfs:comment>
        <rdfs:label>Baggage Handling</rdfs:label>
    </owl:Class>
    


    <!-- http://www.semanticweb.org/prosy/ontologies/2024/3/Airline_Reviews_Ontology#BaggageHandlingRating -->


    <owl:Class rdf:about="http://www.semanticweb.org/prosy/ontologies/2024/3/Airline_Reviews_Ontology#BaggageHandlingRating">
        <rdfs:subClassOf rdf:resource="http://www.semanticweb.org/prosy/ontologies/2024/3/Airline_Reviews_Ontology#BaggageHandling"/>
        <rdfs:comment>A rating that evaluates the effectiveness and care of the airline&apos;s baggage handling services</rdfs:comment>
        <rdfs:label>Baggage Handling Rating</rdfs:label>
    </owl:Class>
    


    <!-- http://www.semanticweb.org/prosy/ontologies/2024/3/Airline_Reviews_Ontology#CabinStaffServiceRating -->


    <owl:Class rdf:about="http://www.semanticweb.org/prosy/ontologies/2024/3/Airline_Reviews_Ontology#CabinStaffServiceRating">
        <rdfs:subClassOf rdf:resource="http://www.semanticweb.org/prosy/ontologies/2024/3/Airline_Reviews_Ontology#ServiceRatings"/>
        <rdfs:comment>A rating for the service provided by the flight&apos;s cabin crew, often out of 5 stars</rdfs:comment>
        <rdfs:label>Cabin Staff Service Rating</rdfs:label>
    </owl:Class>
    


    <!-- http://www.semanticweb.org/prosy/ontologies/2024/3/Airline_Reviews_Ontology#CheckInEfficiency -->


    <owl:Class rdf:about="http://www.semanticweb.org/prosy/ontologies/2024/3/Airline_Reviews_Ontology#CheckInEfficiency">
        <rdfs:subClassOf rdf:resource="http://www.semanticweb.org/prosy/ontologies/2024/3/Airline_Reviews_Ontology#CheckInProcess"/>
        <rdfs:comment>A measure of how quickly and effectively the airline handles check-in procedures</rdfs:comment>
        <rdfs:label>Check-in Efficiency</rdfs:label>
    </owl:Class>
    


    <!-- http://www.semanticweb.org/prosy/ontologies/2024/3/Airline_Reviews_Ontology#CheckInProcess -->


    <owl:Class rdf:about="http://www.semanticweb.org/prosy/ontologies/2024/3/Airline_Reviews_Ontology#CheckInProcess">
        <rdfs:comment>he procedures involved in checking in for a flight at the airport, which can significantly impact passenger satisfaction</rdfs:comment>
        <rdfs:label>Check-in Process</rdfs:label>
    </owl:Class>
    


    <!-- http://www.semanticweb.org/prosy/ontologies/2024/3/Airline_Reviews_Ontology#Company -->


    <owl:Class rdf:about="http://www.semanticweb.org/prosy/ontologies/2024/3/Airline_Reviews_Ontology#Company">
        <rdfs:comment>A business that offers air transportation for both passengers.</rdfs:comment>
        <rdfs:label>Company</rdfs:label>
    </owl:Class>
    


    <!-- http://www.semanticweb.org/prosy/ontologies/2024/3/Airline_Reviews_Ontology#CustomerService -->


    <owl:Class rdf:about="http://www.semanticweb.org/prosy/ontologies/2024/3/Airline_Reviews_Ontology#CustomerService">
        <rdfs:comment>Refers to the overall quality of interaction between the airline staff and the passengers, both on the ground and in-flight</rdfs:comment>
        <rdfs:label>Customer Service</rdfs:label>
    </owl:Class>
    


    <!-- http://www.semanticweb.org/prosy/ontologies/2024/3/Airline_Reviews_Ontology#CustomerServiceRating -->


    <owl:Class rdf:about="http://www.semanticweb.org/prosy/ontologies/2024/3/Airline_Reviews_Ontology#CustomerServiceRating">
        <rdfs:subClassOf rdf:resource="http://www.semanticweb.org/prosy/ontologies/2024/3/Airline_Reviews_Ontology#CustomerService"/>
        <rdfs:comment>A rating that assesses the quality of customer service provided by the airline</rdfs:comment>
        <rdfs:label>Customer Service Rating</rdfs:label>
    </owl:Class>
    


    <!-- http://www.semanticweb.org/prosy/ontologies/2024/3/Airline_Reviews_Ontology#DatePublished -->


    <owl:Class rdf:about="http://www.semanticweb.org/prosy/ontologies/2024/3/Airline_Reviews_Ontology#DatePublished">
        <rdfs:subClassOf rdf:resource="http://www.semanticweb.org/prosy/ontologies/2024/3/Airline_Reviews_Ontology#Identifier"/>
        <rdfs:comment>The date on which the review was published, formatted as YYYY-MM-DD</rdfs:comment>
        <rdfs:label>Date Published</rdfs:label>
    </owl:Class>
    


    <!-- http://www.semanticweb.org/prosy/ontologies/2024/3/Airline_Reviews_Ontology#DestinationAirport -->


    <owl:Class rdf:about="http://www.semanticweb.org/prosy/ontologies/2024/3/Airline_Reviews_Ontology#DestinationAirport">
        <rdfs:subClassOf rdf:resource="http://www.semanticweb.org/prosy/ontologies/2024/3/Airline_Reviews_Ontology#FlightDetails"/>
        <rdfs:comment>The airport at which the flight arrived</rdfs:comment>
        <rdfs:label>Destination Airport</rdfs:label>
    </owl:Class>
    


    <!-- http://www.semanticweb.org/prosy/ontologies/2024/3/Airline_Reviews_Ontology#EnvironmentalConcerns -->


    <owl:Class rdf:about="http://www.semanticweb.org/prosy/ontologies/2024/3/Airline_Reviews_Ontology#EnvironmentalConcerns">
        <rdfs:comment>Issues related to the environmental impact of airline operations, including emissions and sustainability practices</rdfs:comment>
        <rdfs:label>Environmental Concerns</rdfs:label>
    </owl:Class>
    


    <!-- http://www.semanticweb.org/prosy/ontologies/2024/3/Airline_Reviews_Ontology#EnvironmentalInitiativesRating -->


    <owl:Class rdf:about="http://www.semanticweb.org/prosy/ontologies/2024/3/Airline_Reviews_Ontology#EnvironmentalInitiativesRating">
        <rdfs:subClassOf rdf:resource="http://www.semanticweb.org/prosy/ontologies/2024/3/Airline_Reviews_Ontology#EnvironmentalConcerns"/>
        <rdfs:comment>A rating that evaluates the airline&apos;s efforts and practices in reducing its environmental footprint</rdfs:comment>
        <rdfs:label>Environmental Initiatives Rating</rdfs:label>
    </owl:Class>
    


    <!-- http://www.semanticweb.org/prosy/ontologies/2024/3/Airline_Reviews_Ontology#FlightDate -->


    <owl:Class rdf:about="http://www.semanticweb.org/prosy/ontologies/2024/3/Airline_Reviews_Ontology#FlightDate">
        <rdfs:subClassOf rdf:resource="http://www.semanticweb.org/prosy/ontologies/2024/3/Airline_Reviews_Ontology#FlightDetails"/>
        <rdfs:comment>The specific date on which the flight occurred</rdfs:comment>
        <rdfs:label>Flight Date</rdfs:label>
    </owl:Class>
    


    <!-- http://www.semanticweb.org/prosy/ontologies/2024/3/Airline_Reviews_Ontology#FlightDetails -->


    <owl:Class rdf:about="http://www.semanticweb.org/prosy/ontologies/2024/3/Airline_Reviews_Ontology#FlightDetails">
        <rdfs:comment>Information about the flight, including the date and the airports of origin and destination</rdfs:comment>
        <rdfs:label>Flight Details</rdfs:label>
    </owl:Class>
    


    <!-- http://www.semanticweb.org/prosy/ontologies/2024/3/Airline_Reviews_Ontology#FlightTimeliness -->


    <owl:Class rdf:about="http://www.semanticweb.org/prosy/ontologies/2024/3/Airline_Reviews_Ontology#FlightTimeliness">
        <rdfs:comment>Refers to the punctuality of the airline&apos;s flights, including departures and arrivals</rdfs:comment>
        <rdfs:label>Flight Timeliness</rdfs:label>
    </owl:Class>
    


    <!-- http://www.semanticweb.org/prosy/ontologies/2024/3/Airline_Reviews_Ontology#GroundServiceRating -->


    <owl:Class rdf:about="http://www.semanticweb.org/prosy/ontologies/2024/3/Airline_Reviews_Ontology#GroundServiceRating">
        <rdfs:subClassOf rdf:resource="http://www.semanticweb.org/prosy/ontologies/2024/3/Airline_Reviews_Ontology#ServiceRatings"/>
        <rdfs:comment>A rating for the service quality at the airport, such as check-in and baggage handling.</rdfs:comment>
        <rdfs:label>Ground Service Rating</rdfs:label>
    </owl:Class>
    


    <!-- http://www.semanticweb.org/prosy/ontologies/2024/3/Airline_Reviews_Ontology#HighlyRecommended -->


    <owl:Class rdf:about="http://www.semanticweb.org/prosy/ontologies/2024/3/Airline_Reviews_Ontology#HighlyRecommended">
        <rdfs:comment>If a flight receives an overall rating greater than 4 and a cabin service rating also greater than 4, then it is considered highly recommended</rdfs:comment>
        <rdfs:label>HighlyRecommended</rdfs:label>
    </owl:Class>
    


    <!-- http://www.semanticweb.org/prosy/ontologies/2024/3/Airline_Reviews_Ontology#Identifier -->


    <owl:Class rdf:about="http://www.semanticweb.org/prosy/ontologies/2024/3/Airline_Reviews_Ontology#Identifier">
        <rdfs:subClassOf>
            <owl:Restriction>
                <owl:onProperty rdf:resource="http://www.semanticweb.org/prosy/ontologies/2024/3/Airline_Reviews_Ontology#idNumber"/>
                <owl:minQualifiedCardinality rdf:datatype="http://www.w3.org/2001/XMLSchema#nonNegativeInteger">0</owl:minQualifiedCardinality>
                <owl:onDataRange rdf:resource="http://www.w3.org/2002/07/owl#rational"/>
            </owl:Restriction>
        </rdfs:subClassOf>
        <rdfs:subClassOf>
            <owl:Restriction>
                <owl:onProperty rdf:resource="http://www.semanticweb.org/prosy/ontologies/2024/3/Airline_Reviews_Ontology#idNumber"/>
                <owl:maxQualifiedCardinality rdf:datatype="http://www.w3.org/2001/XMLSchema#nonNegativeInteger">9999</owl:maxQualifiedCardinality>
                <owl:onDataRange rdf:resource="http://www.w3.org/2002/07/owl#rational"/>
            </owl:Restriction>
        </rdfs:subClassOf>
        <rdfs:comment>A unique identifier for each review, typically a numeric or alphanumeric string</rdfs:comment>
        <rdfs:label>Identifier</rdfs:label>
        <rdfs:sameAs>https://dbpedia.org/ontology/idNumber</rdfs:sameAs>
    </owl:Class>
    


    <!-- http://www.semanticweb.org/prosy/ontologies/2024/3/Airline_Reviews_Ontology#InflightEntertainmentRating -->


    <owl:Class rdf:about="http://www.semanticweb.org/prosy/ontologies/2024/3/Airline_Reviews_Ontology#InflightEntertainmentRating">
        <rdfs:subClassOf rdf:resource="http://www.semanticweb.org/prosy/ontologies/2024/3/Airline_Reviews_Ontology#InflightServices"/>
        <owl:disjointWith rdf:resource="http://www.semanticweb.org/prosy/ontologies/2024/3/Airline_Reviews_Ontology#Wifi&amp;ConnectivityRating"/>
        <rdfs:comment>A rating evaluating the quality and variety of entertainment options available during the flight</rdfs:comment>
        <rdfs:label>Inflight Entertainment Rating</rdfs:label>
    </owl:Class>
    


    <!-- http://www.semanticweb.org/prosy/ontologies/2024/3/Airline_Reviews_Ontology#InflightServices -->


    <owl:Class rdf:about="http://www.semanticweb.org/prosy/ontologies/2024/3/Airline_Reviews_Ontology#InflightServices">
        <rdfs:comment>Services provided during the flight, including entertainment and connectivity options</rdfs:comment>
        <rdfs:label>Inflight Services</rdfs:label>
    </owl:Class>
    


    <!-- http://www.semanticweb.org/prosy/ontologies/2024/3/Airline_Reviews_Ontology#LowRecomended -->


    <owl:Class rdf:about="http://www.semanticweb.org/prosy/ontologies/2024/3/Airline_Reviews_Ontology#LowRecomended">
        <rdfs:comment>minor than 2</rdfs:comment>
        <rdfs:label>LowRecomended</rdfs:label>
    </owl:Class>
    


    <!-- http://www.semanticweb.org/prosy/ontologies/2024/3/Airline_Reviews_Ontology#LoyaltyProgram -->


    <owl:Class rdf:about="http://www.semanticweb.org/prosy/ontologies/2024/3/Airline_Reviews_Ontology#LoyaltyProgram">
        <rdfs:comment>A program offered by an airline to reward passengers with benefits for frequent travel</rdfs:comment>
        <rdfs:label>Loyalty Program</rdfs:label>
    </owl:Class>
    


    <!-- http://www.semanticweb.org/prosy/ontologies/2024/3/Airline_Reviews_Ontology#LoyaltyProgramBenefits -->


    <owl:Class rdf:about="http://www.semanticweb.org/prosy/ontologies/2024/3/Airline_Reviews_Ontology#LoyaltyProgramBenefits">
        <rdfs:subClassOf rdf:resource="http://www.semanticweb.org/prosy/ontologies/2024/3/Airline_Reviews_Ontology#LoyaltyProgram"/>
        <rdfs:comment>Specific benefits provided to members of the airline&apos;s loyalty program, such as upgrades, extra baggage allowance, or priority boarding</rdfs:comment>
        <rdfs:label>Loyalty Program Benefits</rdfs:label>
    </owl:Class>
    


    <!-- http://www.semanticweb.org/prosy/ontologies/2024/3/Airline_Reviews_Ontology#MaxRating -->


    <owl:Class rdf:about="http://www.semanticweb.org/prosy/ontologies/2024/3/Airline_Reviews_Ontology#MaxRating">
        <rdfs:subClassOf rdf:resource="http://www.semanticweb.org/prosy/ontologies/2024/3/Airline_Reviews_Ontology#Ratings"/>
        <owl:disjointWith rdf:resource="http://www.semanticweb.org/prosy/ontologies/2024/3/Airline_Reviews_Ontology#OverallRating"/>
        <rdfs:comment>The maximum possible rating that can be given</rdfs:comment>
        <rdfs:label>Max Rating</rdfs:label>
    </owl:Class>
    


    <!-- http://www.semanticweb.org/prosy/ontologies/2024/3/Airline_Reviews_Ontology#MiddleRecomended -->


    <owl:Class rdf:about="http://www.semanticweb.org/prosy/ontologies/2024/3/Airline_Reviews_Ontology#MiddleRecomended">
        <rdfs:comment>value between 2 and 4</rdfs:comment>
        <rdfs:label>MiddleRecomended</rdfs:label>
    </owl:Class>
    


    <!-- http://www.semanticweb.org/prosy/ontologies/2024/3/Airline_Reviews_Ontology#OnTimePerformance -->


    <owl:Class rdf:about="http://www.semanticweb.org/prosy/ontologies/2024/3/Airline_Reviews_Ontology#OnTimePerformance">
        <rdfs:subClassOf rdf:resource="http://www.semanticweb.org/prosy/ontologies/2024/3/Airline_Reviews_Ontology#FlightTimeliness"/>
        <rdfs:comment>A rating that measures how often the airline&apos;s flights operate on schedule</rdfs:comment>
        <rdfs:label>On-time Performance</rdfs:label>
    </owl:Class>
    


    <!-- http://www.semanticweb.org/prosy/ontologies/2024/3/Airline_Reviews_Ontology#OriginAirport -->


    <owl:Class rdf:about="http://www.semanticweb.org/prosy/ontologies/2024/3/Airline_Reviews_Ontology#OriginAirport">
        <rdfs:subClassOf rdf:resource="http://www.semanticweb.org/prosy/ontologies/2024/3/Airline_Reviews_Ontology#FlightDetails"/>
        <rdfs:comment>The airport from which the flight departed</rdfs:comment>
        <rdfs:label>Origin Airport</rdfs:label>
    </owl:Class>
    


    <!-- http://www.semanticweb.org/prosy/ontologies/2024/3/Airline_Reviews_Ontology#OverallRating -->


    <owl:Class rdf:about="http://www.semanticweb.org/prosy/ontologies/2024/3/Airline_Reviews_Ontology#OverallRating">
        <rdfs:subClassOf rdf:resource="http://www.semanticweb.org/prosy/ontologies/2024/3/Airline_Reviews_Ontology#Ratings"/>
        <rdfs:comment>A general rating given by the reviewer to the airline</rdfs:comment>
        <rdfs:label>Overall Rating</rdfs:label>
    </owl:Class>
    


    <!-- http://www.semanticweb.org/prosy/ontologies/2024/3/Airline_Reviews_Ontology#Ratings -->


    <owl:Class rdf:about="http://www.semanticweb.org/prosy/ontologies/2024/3/Airline_Reviews_Ontology#Ratings">
        <rdfs:subClassOf>
            <owl:Restriction>
                <owl:onProperty rdf:resource="http://www.semanticweb.org/prosy/ontologies/2024/3/Airline_Reviews_Ontology#overallRating"/>
                <owl:minQualifiedCardinality rdf:datatype="http://www.w3.org/2001/XMLSchema#nonNegativeInteger">0</owl:minQualifiedCardinality>
                <owl:onDataRange rdf:resource="http://www.w3.org/2002/07/owl#rational"/>
            </owl:Restriction>
        </rdfs:subClassOf>
        <rdfs:subClassOf>
            <owl:Restriction>
                <owl:onProperty rdf:resource="http://www.semanticweb.org/prosy/ontologies/2024/3/Airline_Reviews_Ontology#overallRating"/>
                <owl:maxQualifiedCardinality rdf:datatype="http://www.w3.org/2001/XMLSchema#nonNegativeInteger">10</owl:maxQualifiedCardinality>
                <owl:onDataRange rdf:resource="http://www.w3.org/2002/07/owl#rational"/>
            </owl:Restriction>
        </rdfs:subClassOf>
        <rdfs:comment>Contains all ratings associated with the review, including overall, service, and specific amenities</rdfs:comment>
        <rdfs:label>Ratings</rdfs:label>
    </owl:Class>
    


    <!-- http://www.semanticweb.org/prosy/ontologies/2024/3/Airline_Reviews_Ontology#Recommendation -->


    <owl:Class rdf:about="http://www.semanticweb.org/prosy/ontologies/2024/3/Airline_Reviews_Ontology#Recommendation">
        <rdfs:comment>Indicates whether the review author recommends the airline service to other potential customers</rdfs:comment>
        <rdfs:label>Recommendation</rdfs:label>
    </owl:Class>
    


    <!-- http://www.semanticweb.org/prosy/ontologies/2024/3/Airline_Reviews_Ontology#RecommendationStatus -->


    <owl:Class rdf:about="http://www.semanticweb.org/prosy/ontologies/2024/3/Airline_Reviews_Ontology#RecommendationStatus">
        <rdfs:subClassOf rdf:resource="http://www.semanticweb.org/prosy/ontologies/2024/3/Airline_Reviews_Ontology#Recommendation"/>
        <rdfs:comment>A boolean value indicating if the airline is recommended by the reviewer</rdfs:comment>
        <rdfs:label>Recommendation Status</rdfs:label>
    </owl:Class>
    


    <!-- http://www.semanticweb.org/prosy/ontologies/2024/3/Airline_Reviews_Ontology#ReviewBody -->


    <owl:Class rdf:about="http://www.semanticweb.org/prosy/ontologies/2024/3/Airline_Reviews_Ontology#ReviewBody">
        <rdfs:subClassOf rdf:resource="http://www.semanticweb.org/prosy/ontologies/2024/3/Airline_Reviews_Ontology#ReviewContent"/>
        <owl:disjointWith rdf:resource="http://www.semanticweb.org/prosy/ontologies/2024/3/Airline_Reviews_Ontology#ReviewTitle"/>
        <rdfs:comment>The main textual content of the review</rdfs:comment>
        <rdfs:label>Review Body</rdfs:label>
    </owl:Class>
    


    <!-- http://www.semanticweb.org/prosy/ontologies/2024/3/Airline_Reviews_Ontology#ReviewContent -->


    <owl:Class rdf:about="http://www.semanticweb.org/prosy/ontologies/2024/3/Airline_Reviews_Ontology#ReviewContent">
        <rdfs:comment>Contains the main textual content of the review, including the title and body</rdfs:comment>
        <rdfs:label>Review Content</rdfs:label>
    </owl:Class>
    


    <!-- http://www.semanticweb.org/prosy/ontologies/2024/3/Airline_Reviews_Ontology#ReviewTitle -->


    <owl:Class rdf:about="http://www.semanticweb.org/prosy/ontologies/2024/3/Airline_Reviews_Ontology#ReviewTitle">
        <rdfs:subClassOf rdf:resource="http://www.semanticweb.org/prosy/ontologies/2024/3/Airline_Reviews_Ontology#ReviewContent"/>
        <rdfs:comment>The title of the review</rdfs:comment>
        <rdfs:label>Review Title</rdfs:label>
    </owl:Class>
    


    <!-- http://www.semanticweb.org/prosy/ontologies/2024/3/Airline_Reviews_Ontology#Safety -->


    <owl:Class rdf:about="http://www.semanticweb.org/prosy/ontologies/2024/3/Airline_Reviews_Ontology#Safety">
        <rdfs:comment>Aspects of airline operations that concern the safety and security of passengers and crew during flights</rdfs:comment>
        <rdfs:label>Safety</rdfs:label>
    </owl:Class>
    


    <!-- http://www.semanticweb.org/prosy/ontologies/2024/3/Airline_Reviews_Ontology#SafetyMeasuresRating -->


    <owl:Class rdf:about="http://www.semanticweb.org/prosy/ontologies/2024/3/Airline_Reviews_Ontology#SafetyMeasuresRating">
        <rdfs:subClassOf rdf:resource="http://www.semanticweb.org/prosy/ontologies/2024/3/Airline_Reviews_Ontology#Safety"/>
        <rdfs:comment>A rating that assesses the effectiveness of the safety measures and protocols implemented by the airline</rdfs:comment>
        <rdfs:label>Safety Measures Rating</rdfs:label>
    </owl:Class>
    


    <!-- http://www.semanticweb.org/prosy/ontologies/2024/3/Airline_Reviews_Ontology#SeatComfortRating -->


    <owl:Class rdf:about="http://www.semanticweb.org/prosy/ontologies/2024/3/Airline_Reviews_Ontology#SeatComfortRating">
        <rdfs:subClassOf rdf:resource="http://www.semanticweb.org/prosy/ontologies/2024/3/Airline_Reviews_Ontology#SeatDetails"/>
        <owl:disjointWith rdf:resource="http://www.semanticweb.org/prosy/ontologies/2024/3/Airline_Reviews_Ontology#SeatType"/>
        <rdfs:comment>A rating of the comfort of the seat</rdfs:comment>
        <rdfs:label>Seat Comfort Rating</rdfs:label>
    </owl:Class>
    


    <!-- http://www.semanticweb.org/prosy/ontologies/2024/3/Airline_Reviews_Ontology#SeatDetails -->


    <owl:Class rdf:about="http://www.semanticweb.org/prosy/ontologies/2024/3/Airline_Reviews_Ontology#SeatDetails">
        <rdfs:comment>Details about the seating on the flight, including type and comfort rating</rdfs:comment>
        <rdfs:label>Seat Details</rdfs:label>
    </owl:Class>
    


    <!-- http://www.semanticweb.org/prosy/ontologies/2024/3/Airline_Reviews_Ontology#SeatType -->


    <owl:Class rdf:about="http://www.semanticweb.org/prosy/ontologies/2024/3/Airline_Reviews_Ontology#SeatType">
        <rdfs:subClassOf rdf:resource="http://www.semanticweb.org/prosy/ontologies/2024/3/Airline_Reviews_Ontology#SeatDetails"/>
        <rdfs:comment>The type of seat chosen on the flight</rdfs:comment>
        <rdfs:label>Seat Type</rdfs:label>
    </owl:Class>
    


    <!-- http://www.semanticweb.org/prosy/ontologies/2024/3/Airline_Reviews_Ontology#ServiceRatings -->


    <owl:Class rdf:about="http://www.semanticweb.org/prosy/ontologies/2024/3/Airline_Reviews_Ontology#ServiceRatings">
        <rdfs:comment>Ratings related to specific services provided during the flight, including cabin staff and ground service</rdfs:comment>
        <rdfs:label>Service Ratings</rdfs:label>
    </owl:Class>
    


    <!-- http://www.semanticweb.org/prosy/ontologies/2024/3/Airline_Reviews_Ontology#TripVerified -->


    <owl:Class rdf:about="http://www.semanticweb.org/prosy/ontologies/2024/3/Airline_Reviews_Ontology#TripVerified">
        <rdfs:subClassOf rdf:resource="http://www.semanticweb.org/prosy/ontologies/2024/3/Airline_Reviews_Ontology#Verification"/>
        <owl:disjointWith rdf:resource="http://www.semanticweb.org/prosy/ontologies/2024/3/Airline_Reviews_Ontology#Verified"/>
        <rdfs:comment>Indicates whether the travel review has been verified by the airline or a third party as a genuine experience</rdfs:comment>
        <rdfs:label>Trip Verified</rdfs:label>
    </owl:Class>
    


    <!-- http://www.semanticweb.org/prosy/ontologies/2024/3/Airline_Reviews_Ontology#ValueAssessment -->


    <owl:Class rdf:about="http://www.semanticweb.org/prosy/ontologies/2024/3/Airline_Reviews_Ontology#ValueAssessment">
        <rdfs:comment>Assesses the value for money of the flight experience</rdfs:comment>
        <rdfs:label>Value Assessment</rdfs:label>
    </owl:Class>
    


    <!-- http://www.semanticweb.org/prosy/ontologies/2024/3/Airline_Reviews_Ontology#ValueForMoneyRating -->


    <owl:Class rdf:about="http://www.semanticweb.org/prosy/ontologies/2024/3/Airline_Reviews_Ontology#ValueForMoneyRating">
        <rdfs:subClassOf rdf:resource="http://www.semanticweb.org/prosy/ontologies/2024/3/Airline_Reviews_Ontology#ValueAssessment"/>
        <rdfs:comment>Rating that evaluates the overall value for money of the flight</rdfs:comment>
        <rdfs:label>Value For Money Rating</rdfs:label>
    </owl:Class>
    


    <!-- http://www.semanticweb.org/prosy/ontologies/2024/3/Airline_Reviews_Ontology#Verification -->


    <owl:Class rdf:about="http://www.semanticweb.org/prosy/ontologies/2024/3/Airline_Reviews_Ontology#Verification">
        <rdfs:comment>Indicates the verification status of the review, determining if it reflects a verified travel experience</rdfs:comment>
        <rdfs:label>Verification</rdfs:label>
    </owl:Class>
    


    <!-- http://www.semanticweb.org/prosy/ontologies/2024/3/Airline_Reviews_Ontology#Verified -->


    <owl:Class rdf:about="http://www.semanticweb.org/prosy/ontologies/2024/3/Airline_Reviews_Ontology#Verified">
        <rdfs:subClassOf rdf:resource="http://www.semanticweb.org/prosy/ontologies/2024/3/Airline_Reviews_Ontology#Verification"/>
        <rdfs:comment>A status that shows whether the review has been authenticated as coming from an actual passenger</rdfs:comment>
        <rdfs:label>Verified</rdfs:label>
    </owl:Class>
    


    <!-- http://www.semanticweb.org/prosy/ontologies/2024/3/Airline_Reviews_Ontology#Food&amp;BeveragesRating -->


    <owl:Class rdf:about="http://www.semanticweb.org/prosy/ontologies/2024/3/Airline_Reviews_Ontology#Food&amp;BeveragesRating">
        <rdfs:subClassOf rdf:resource="http://www.semanticweb.org/prosy/ontologies/2024/3/Airline_Reviews_Ontology#ServiceRatings"/>
        <rdfs:comment>A rating for the quality of food and beverages offered during the flight</rdfs:comment>
        <rdfs:label>Food &amp; Beverages Rating</rdfs:label>
    </owl:Class>
    


    <!-- http://www.semanticweb.org/prosy/ontologies/2024/3/Airline_Reviews_Ontology#Wifi&amp;ConnectivityRating -->


    <owl:Class rdf:about="http://www.semanticweb.org/prosy/ontologies/2024/3/Airline_Reviews_Ontology#Wifi&amp;ConnectivityRating">
        <rdfs:subClassOf rdf:resource="http://www.semanticweb.org/prosy/ontologies/2024/3/Airline_Reviews_Ontology#InflightServices"/>
        <rdfs:comment>A rating assessing the availability and quality of WiFi and other connectivity services on board</rdfs:comment>
        <rdfs:label>Wifi &amp; Connectivity Rating</rdfs:label>
    </owl:Class>
    


    <!-- 
    ///////////////////////////////////////////////////////////////////////////////////////
    //
    // Individuals
    //
    ///////////////////////////////////////////////////////////////////////////////////////
     -->


    


    <!-- http://www.semanticweb.org/prosy/ontologies/2024/3/Airline_Reviews_Ontology#Boing737_900 -->


    <owl:NamedIndividual rdf:about="http://www.semanticweb.org/prosy/ontologies/2024/3/Airline_Reviews_Ontology#Boing737_900">
        <rdf:type rdf:resource="http://www.semanticweb.org/prosy/ontologies/2024/3/Airline_Reviews_Ontology#AircraftDetails"/>
        <usesAircraft rdf:resource="http://www.semanticweb.org/prosy/ontologies/2024/3/Airline_Reviews_Ontology#Boing737_900"/>
        <rdfs:comment>This instance represents the Boeing 737 Dreamliner, a long-haul, mid-size widebody, twin-engine jet airliner. Known for its fuel efficiency and advanced technology, it is designed to provide airlines with better efficiency and passengers with a more comfortable flying experience. It features innovations such as electrical flight systems, composite materials, and larger windows</rdfs:comment>
        <rdfs:label>Boing737_900</rdfs:label>
        <rdfs:sameAs>https://dbpedia.org/page/Boeing_737_Next_Generation</rdfs:sameAs>
    </owl:NamedIndividual>
    


    <!-- http://www.semanticweb.org/prosy/ontologies/2024/3/Airline_Reviews_Ontology#EconomyClass -->


    <owl:NamedIndividual rdf:about="http://www.semanticweb.org/prosy/ontologies/2024/3/Airline_Reviews_Ontology#EconomyClass">
        <rdf:type rdf:resource="http://www.semanticweb.org/prosy/ontologies/2024/3/Airline_Reviews_Ontology#SeatDetails"/>
        <hasSeat rdf:resource="http://www.semanticweb.org/prosy/ontologies/2024/3/Airline_Reviews_Ontology#EconomyClass"/>
        <rdfs:comment>Economy class individual</rdfs:comment>
        <rdfs:label>Economy Class</rdfs:label>
    </owl:NamedIndividual>
    


    <!-- http://www.semanticweb.org/prosy/ontologies/2024/3/Airline_Reviews_Ontology#ID5235 -->


    <owl:NamedIndividual rdf:about="http://www.semanticweb.org/prosy/ontologies/2024/3/Airline_Reviews_Ontology#ID5235">
        <rdf:type rdf:resource="http://www.semanticweb.org/prosy/ontologies/2024/3/Airline_Reviews_Ontology#Identifier"/>
        <hasAuthor rdf:resource="http://www.semanticweb.org/prosy/ontologies/2024/3/Airline_Reviews_Ontology#MaryLe"/>
        <idNumber>ID5235</idNumber>
        <rdfs:comment>ID5283 is the unique identifier used in the database to locate user reviews</rdfs:comment>
        <rdfs:label>ID5235</rdfs:label>
    </owl:NamedIndividual>
    


    <!-- http://www.semanticweb.org/prosy/ontologies/2024/3/Airline_Reviews_Ontology#MaryLe -->


    <owl:NamedIndividual rdf:about="http://www.semanticweb.org/prosy/ontologies/2024/3/Airline_Reviews_Ontology#MaryLe">
        <rdf:type rdf:resource="http://www.semanticweb.org/prosy/ontologies/2024/3/Airline_Reviews_Ontology#Author"/>
        <hasFlightDetails rdf:resource="http://www.semanticweb.org/prosy/ontologies/2024/3/Airline_Reviews_Ontology#Boing737_900"/>
        <rdfs:comment>A frequent Economy Class traveler flying from Tokyo to London Heathrow via Doha.</rdfs:comment>
        <rdfs:label>Mary Le</rdfs:label>
    </owl:NamedIndividual>
    


    <!-- http://www.semanticweb.org/prosy/ontologies/2024/3/Airline_Reviews_Ontology#Qatar_Airways -->


    <owl:NamedIndividual rdf:about="http://www.semanticweb.org/prosy/ontologies/2024/3/Airline_Reviews_Ontology#Qatar_Airways">
        <rdf:type rdf:resource="http://www.semanticweb.org/prosy/ontologies/2024/3/Airline_Reviews_Ontology#Company"/>
        <rdfs:comment>Qatar Airways is the national airline of the State of Qatar and one of the leading airlines in the world, known for its high levels of service excellence. Here are some key points about Qatar Airways:</rdfs:comment>
        <rdfs:label>Qatar Airways</rdfs:label>
        <rdfs:sameAs>http://dbpedia.org/resource/Qatar_Airways</rdfs:sameAs>
    </owl:NamedIndividual>
    


    <!-- http://www.semanticweb.org/prosy/ontologies/2024/3/Airline_Reviews_Ontology#Ryanair -->


    <owl:NamedIndividual rdf:about="http://www.semanticweb.org/prosy/ontologies/2024/3/Airline_Reviews_Ontology#Ryanair">
        <rdf:type rdf:resource="http://www.semanticweb.org/prosy/ontologies/2024/3/Airline_Reviews_Ontology#Company"/>
        <rdfs:comment>Ryanair company</rdfs:comment>
        <rdfs:label>Ryanair</rdfs:label>
        <rdfs:sameAs>https://dbpedia.org/page/Ryanair</rdfs:sameAs>
    </owl:NamedIndividual>
    


    <!-- http://www.semanticweb.org/prosy/ontologies/2024/3/Airline_Reviews_Ontology#1.0 -->


    <owl:NamedIndividual rdf:about="http://www.semanticweb.org/prosy/ontologies/2024/3/Airline_Reviews_Ontology#1.0">
        <rdf:type rdf:resource="http://www.semanticweb.org/prosy/ontologies/2024/3/Airline_Reviews_Ontology#Ratings"/>
        <hasRating rdf:resource="http://www.semanticweb.org/prosy/ontologies/2024/3/Airline_Reviews_Ontology#1.0"/>
        <rdfs:comment>Value of rating by author</rdfs:comment>
        <rdfs:label rdf:datatype="http://www.w3.org/2001/XMLSchema#decimal">1.0</rdfs:label>
    </owl:NamedIndividual>
    


    <!-- 
    ///////////////////////////////////////////////////////////////////////////////////////
    //
    // General axioms
    //
    ///////////////////////////////////////////////////////////////////////////////////////
     -->


    <rdf:Description>
        <rdf:type rdf:resource="http://www.w3.org/2002/07/owl#AllDisjointClasses"/>
        <owl:members rdf:parseType="Collection">
            <rdf:Description rdf:about="http://www.semanticweb.org/prosy/ontologies/2024/3/Airline_Reviews_Ontology#CabinStaffServiceRating"/>
            <rdf:Description rdf:about="http://www.semanticweb.org/prosy/ontologies/2024/3/Airline_Reviews_Ontology#GroundServiceRating"/>
            <rdf:Description rdf:about="http://www.semanticweb.org/prosy/ontologies/2024/3/Airline_Reviews_Ontology#Food&amp;BeveragesRating"/>
        </owl:members>
    </rdf:Description>
    <rdf:Description>
        <rdf:type rdf:resource="http://www.w3.org/2002/07/owl#AllDisjointClasses"/>
        <owl:members rdf:parseType="Collection">
            <rdf:Description rdf:about="http://www.semanticweb.org/prosy/ontologies/2024/3/Airline_Reviews_Ontology#DestinationAirport"/>
            <rdf:Description rdf:about="http://www.semanticweb.org/prosy/ontologies/2024/3/Airline_Reviews_Ontology#FlightDate"/>
            <rdf:Description rdf:about="http://www.semanticweb.org/prosy/ontologies/2024/3/Airline_Reviews_Ontology#OriginAirport"/>
        </owl:members>
    </rdf:Description>
</rdf:RDF>



<!-- Generated by the OWL API (version 5.1.18) https://github.com/owlcs/owlapi/ -->


